Author: Kevin Xu
==Note: I forgot you can use calculators! Thus some calculation steps can just be ignored :)==
### Part A

P1: $2^r = 16, r = 4$ and $5^2 = 25, s = 2$ so $r+s = 4+2 = \boxed{6}$.

P2: Note $x^2-y^2 = (x+y)(x-y)$. We have $5 \cdot 2 = \frac{(x+y)}{2} \cdot \frac{(x-y)}{2} = \frac{(x+y)(x-y)}{4} = \frac{x^2-y^2}{4}$. Thus, $10 \cdot 4 = x^2-y^2 = \boxed{40}$.

P3: LCM calls for prime factoring, $273 = 3 \cdot 7 \cdot 13$ (Note that $91 = 7 \cdot 13$). This means that the two numbers uses each of $3,7,13$ in its prime factor at most once, and each is used at least once. 
Here, we may have two approaches.
First approach (systematic): Looking at the number with $13$ in it's factor, we can either have $13$ or $13 \cdot 3$ as the number since $13 \cdot 7 = 91 > 60$. If $13$, the other number is $3 \cdot 7 = 21$ (because if $3 \cdot 7 \cdot 13$, it will obviously exceed) but $21 +13 = 34$ so no. If $13 \cdot 3$, we may have $7$ or $7 \cdot 3$. We see that $13 \cdot 3 + 7 \cdot 3 = 39 + 21 = 60$, so we're done.
Second approach (intuition): just look and see that the numbers can't be further apart and be somewhat small. We can see $3 \cdot 7 = 21, 3 \cdot 13 = 39$ so it has to be $21 + 39 = 60$.
The two numbers are $\boxed{21,39}$.

P4: By Pythagorean Theorem, $CD = \sqrt{625^2 - 600^2} = \sqrt{(625+600)(625-600)} = \sqrt{(1225)(25)} = 7 \cdot 25 = 175$ (btw we may also just do this by seeing that $\frac{600}{625} = \frac{24}{25}$ so it's a 7-24-25 right triangle, so $CD = 25 \cdot 7$).
The other information they give is the angle relation. To relate angles to lengths, we use Trig functions. We have $\sin(\angle BAC) = \sin(2 \angle DAC) = 2\sin(\angle DAC)\cos(\angle DAC)$. Since we know all the lengths for $\triangle ADC$, we get $\sin(\angle DAC) = \frac{175}{625} = \frac{7}{25}$ and $\cos(\angle DAC) = \frac{600}{625} = \frac{24}{25}$. Thus, $\sin(\angle BAC) = \sin(2\angle DAC) = 2 \cdot \frac{7}{25} \cdot \frac{24}{25} = \frac{336}{625}$. Moreover, $\sin(\angle BAC) = \frac{opp}{hyp} = \frac{BC}{AC} = \frac{BC}{625}$. Thus, $BC = \boxed{336}$.

P5: Note that any point on a circle forms a right angle  with it's diameter. Thus, $\angle ARB = 90^{\circ}$. We want to try to put as many lengths in terms of $AP = x$ as possible so that we can get some equality and solve. We take advantage of right angles and use Pythagorean Theorem to find length. Since $\angle ARB = 90^{\circ}, \angle ARQ = 90^{\circ}$. Since $\angle APQ = \angle PQB = \angle ARQ = 90^{\circ}$, $PARQ$ is a rectangle. Thus, $AP = QR \rightarrow AP = RB$. $(CD+2) = \sqrt{AB^2-RB^2}= \sqrt{76-x^2}, CD=\sqrt{76-x^2}-2$.  $AD= \sqrt{x^2+(CD+1)^2}, DB = \sqrt{1^2 +(2x)^2} = \sqrt{4x^2+1}$.  Then, $AD = \sqrt{76 - (4x^2+1)} = \sqrt{75-4x^2}$. Thus, 
$$
\begin{align}
x^2+(\sqrt{76-x^2}-1)^2 &= 75-4x^2 \\
x^2+(76-x^2) -2\sqrt{76-x^2}+1 &= 77-2\sqrt{76-x^2} = 75-4x^2 \\
2x^2+1 &= \sqrt{76-x^2} \\
4x^4+4x^2+1 &= 76-x^2 \\
4x^4+5x^2-75 &= 0 \\
x^2 = -5,\frac{15}{4}.
\end{align}
$$
Since the square of a number can't be negative, $x^2 = \frac{15}{4}, x = \pm \frac{\sqrt{15}}{2}$. 
Since $x$ is not negative, $x = \boxed{\frac{\sqrt{15}}{2}}$.

P6: We view this as placing the marbles in a line, where there are 15 spots. In total, the number of ways to put these balls in place is 
$$
\begin{align}
\binom{15}{3} \cdot \binom{12}{5} &= \frac{15 \cdot 14 \cdot 13}{6} \cdot \frac{12 \cdot 11 \cdot 10 \cdot 9 \cdot 8}{120} \\
&= 15 \cdot 14 \cdot 13 \cdot 11 \cdot 3 \cdot 4 \\
&= 60 \cdot 154 \cdot 39 \\
&= 60 \cdot 6006\\
&= 360360.
\end{align}
$$Note we didn't count the last color since after putting in red and blue, there is only 7 spots for green so there's one way. 
We want all cases such that the last red marble comes before the last green and blue marble. Let's look at the last marble of each color. Note that the last marble in line must be either blue or green. Thus, we have two cases.

First case: let the last be green (then we can do same for other case and get the same answer). We can view green as a "filler", meaning we don't care about where it goes, after filling in red and blue, green will fall into place so there's one way. Ok, let the red and blue endpoint indexes be $a$ and $b$ respectively, where $a<b$. Note that $3 \le a \le 13$ since we must save $3$ spots for red and we need to make room for last blue and last green so $15-1-1= 13$,and $8 \le b \le 14$ since $3+5=8$ spots for red and blue and save last spot for green so $15-1 = 14$. Then, the other $2$ red marbles must be before index $a$ and the other $4$ blue marbles must be before index $b$. Thus, number of ways for this specific $(a,b)$ is $\binom{a-1}{2} \cdot \binom{b-1-3}{4}$. Then, everything else can only be filled with green marbles. Then, we want the sum of every $a,b$ possible. Thus, total ways where the last marble is green is
$$
\begin{align}
\sum_{a=3}^{13} \sum_{b=8}^{14} \left(\binom{a-1}{2} \cdot \binom{b-4}{4}\right) &= \sum_{a=3}^{13} \left( \binom{a-1}{2} \cdot \sum_{b=8}^{14}  \binom{b-4}{4}\right) \\
&= \left( \sum_{a=3}^{13}  \binom{a-1}{2} \right) \cdot \left( \sum_{b=8}^{14}  \binom{b-4}{4} \right) \\
&= \left( \sum_{a=2}^{12}  \binom{a}{2} \right) \cdot \left( \sum_{b=4}^{10}  \binom{b}{4}\right) \\
\end{align}
$$
By Hockey Stick Theorem in [[Combo Identities]], $\sum_{i=k}^{n} \binom{i}{k} = \binom{n+1}{k+1}$ for all integers $n$ and $k$. Thus, 
$$
\begin{align}
\sum_{a=2}^{12} \binom{a}{2} = \binom{13}{3}, \sum_{b=4}^{10}  \binom{b}{4} &= \binom{11}{5} \\
\left( \sum_{a=2}^{12}  \binom{a}{2} \right) \cdot \left( \sum_{b=4}^{10}  \binom{b}{4}\right) &= \binom{13}{3} \cdot \binom{11}{5} \\ 
&= \frac{13 \cdot 12 \cdot 11}{6} \cdot \frac{11 \cdot 10 \cdot 9 \cdot 8 \cdot 7}{120} \\
&= 13 \cdot 11 \cdot 11 \cdot 3 \cdot 4 \cdot 7 \\ 
&= 143 \cdot 924 \\
&= 132132.
\end{align}
$$

Second case: Let last be blue. This is similar to first case. Red remains the same so we have $\binom{a-1}{2}$ ways. For green, there are 7 marbles. So $10 \le b \le 14$ since $3+7 = 10$ and $15-1 = 14$. Number of ways for specific $a,b$ is $\binom{a-1}{2} \cdot \binom{b-1-3}{6}$. Thus, 
$$
\begin{align}
\sum_{a=3}^{13} \sum_{b=10}^{14} \left(\binom{a-1}{2} \cdot \binom{b-4}{6}\right) &= \left( \sum_{a=2}^{12}  \binom{a}{2} \right) \cdot \left( \sum_{b=6}^{10}  \binom{b}{6}\right) \\
&= \binom{13}{3} \cdot \binom{11}{7} \\
&= \binom{13}{3} \cdot \binom{11}{4} \\
&= \frac{13 \cdot 12 \cdot 11}{6} \cdot \frac{11 \cdot 10 \cdot 9 \cdot 8 }{24} \\
&= 13 \cdot 11 \cdot 11 \cdot 10 \cdot 3 \cdot 2 \\ 
&= 1210 \cdot 78 \\
&= 94380.
\end{align}
$$
All together, the probability is 
$$
\begin{align}
\frac{\textnormal{desired outcome}}{\textnormal{total outcome}} &= \frac{132132 + 94380}{360360} \\
&= \frac{226512}{360360} \\
&= \boxed{\frac{44}{91}}.
\end{align}
$$



### Part B

P1: 

P2: 
a) $a^2+a = \frac{4}{9}, a^2+a-\frac{4}{9} = 0, a = -\frac{1}{3}, \frac{4}{3}$. Thus, $a = \boxed{\frac{4}{3}}$.

b) $m^2 + m + \frac{1}{4} + m+\frac{1}{2}$, $m^2 + 2m + \frac{3}{4} = (m+1)^2 - \frac{1}{4}$. Thus, $(m+1)^2- ((m+1)^2 - \frac{1}{4}) = \boxed{\frac{1}{4}}$ for all positive integer $m$.

c) Since they are all positive, $n^2 < c+\sqrt{c} < (n+1)^2$. If $a$ is the smallest such $c$ and $b$ is the largest such $c$. It will be even if and only if $b-a$ is odd since everything in between $a$ and $b$ must also satisfy the inequality. The largest $c$ must have $n \le \sqrt{c} <n+1$. If $\sqrt{c} < n,  

P3: 
a) 
