P1: $|x| \le 9$ so $\boxed{D) \space 19}$.

P2: $46$ people in blue-blue pairs, $57-46 = 11$ people in blue-yellow pairs, $66-23-11 = \boxed{B) \space 32}$.

P3: $\frac{1}{1 + \frac{1}{2+ \frac{2}{3+x}}} = \frac{38}{53}, 1 + \frac{1}{2+ \frac{2}{3+x}} = \frac{53}{38},\frac{1}{2+ \frac{2}{3+x}} = \frac{15}{38}, 2+ \frac{2}{3+x} =\frac{38}{15}, \frac{8}{15}=\frac{2}{3+x},8(3+x) =30, x = \boxed{A) \space \frac{3}{4}}$.

P4: $\frac{84 \cdot 3x + 70 \cdot 4x}{7x} = \frac{532x}{7x} = \boxed{C) \space 76}$.

P5: Work backwards by geometry (==idk how to approach by algebra==) $(-6,3) \rightarrow (-3,6) \rightarrow (2,9)$. $9-2 = \boxed{D) \space 7}$.

P6: $\frac{1}{3} \pi 12^2 \cdot 18 = 6 \cdot 144 \pi$. $864\pi \div 24^2 \pi = \boxed{A) \space 1.5}$.

P7: $N = 2^3 \cdot ...$ $1: (2^0 + 2^1 + 2^2 + 2^3) = \boxed{B) \space 1:15}$.

P8: $r^2 = (\frac{1}{2}x)^2 + 19^2 = (\frac{3}{2}x)^2 + 17^2, 2x^2 = 19^2-17^2, x = \boxed{B) \space 6}$ 

P9: We want common base. By [[Logorithm]], $\frac{\log_2{80}}{\frac{1}{\log_2{40}}} - \frac{log_2{160}}{\frac{1}{\log_2{20}}}$. We can thus put everything in terms of $x = \log_2{20}$. $(\log_2{20}+2)(\log_2{20}+1) - (\log_2{20}+3)(\log_2{20}) = \boxed{D) \space 2}$.

P10: $\frac{37\cdot 38}{2} -a-b = 703-a-b = ab, 704 = (a+1)(b+1) = 2^6 \cdot 11$. Two numbers are $32 \cdot 22, a = 31, b = 21, 31-21 = \boxed{E) \space 10}$.

P11: Refer to diagram in solutions. $AD =\frac{BC}{2} = 7$ and $EC = 2(AB) = 26$. Moreover, $2PD=BP$ and $2BP = PE$. We thus evoke [[Stuart's Theorem]] on $\triangle ABD$. We have $6x^3 + 5^2(3x) = 7^2(2x) + 13^2(x), x = 4\sqrt{2}$. $DE = PE - PD = 4x - x = 3x = \boxed{D) \space 12\sqrt{2}}$.

P12: Let least integer be $x$. $x = 32(s-1) - 35(s-2) = 38-3s$. $x+72 = 40(s-1) - 35(s-2) = 5s+30$. Thus, $72 = 8s - 8, s= 10, x = 8$. Largest integer is $x+72 = 80$. $\frac{32(s-1) + 80}{s} = \boxed{D) \space 36.8}$.

P13: $5 \cos{3 \theta} = 3 \sin{\theta} - 1$. We can graph these two function easily. 

P14: Let $DM = x$ and side lengths of $ABCD$ be $a$ and $b$. $\sqrt{a^2 + x^2} = \sqrt{b^2+x^2}-2,\sqrt{b^2+x^2}+2  = \sqrt{(a^2+b^2)+x^2}$.
 